proof/myset.ec
@@ -6,18 +6,29 @@ lemma mem_rm: forall (y:'a) (x:'a) (S:'a set),
   x <> y =>
   mem y (rm x S) = mem y S by [].
 
-(*
 lemma mem_map: forall (f:'a -> 'b) xs x,
-  mem x xs =>
-  mem (f x) (map f xs) by (intros _ S x _;elimT induction_det S;trivial).*)
+  Set.mem x xs =>
+  Set.mem (f x) (map f xs).
+intros f S x;elimT Set.Induction.induction_det S;first smt.
+simplify.
+intros S0 hrec h.
+rewrite (map_cons<:'b,'a> f S0).
+smt.
+save.
+
+
+lemma mem_map_rev: forall (f:'a -> 'b) xs x,
+  Set.mem (f x) (Set.map f xs) =>
+  (exists y, f x = f y /\ Set.mem y xs)
+by (intros _ S _;elimT Set.Induction.induction_det S;smt).
 
 (*
 lemma _map_add: forall (f:'a -> 'b) x xs,
   !(mem x xs) =>
   map f (add x xs) = add (f x) (map f xs).
   intros f x xs h.
-  rewrite (map_cons<:'b, 'a> f (add x xs));first trivial.
-  rewrite (_ : rm x (add x xs) = xs);first trivial.
+  rewrite (map_cons<:'b, 'a> f (add x xs));first smt.
+  rewrite (_ : rm x (add x xs) = xs);first smt.
   split.
 save.
 *)
@@ -30,205 +41,70 @@ lemma map_add: forall (f:'a -> 'b) xs,
   case (mem x xs);last (apply _map_add;first assumption).
   intros hh.
   rewrite <- (mem_add<:'a> x xs _);first assumption.
-  rewrite <- (mem_add<:'b> (f x) (map f xs) _);trivial.
+  rewrite <- (mem_add<:'b> (f x) (map f xs) _);smt.
 save.
 *)
 
 (*
 lemma mem_map_bij: forall (f:'a -> 'b) x xs,
   (forall x y, f x = f y => x = y) =>
-  mem x xs = mem (f x) (map f xs) by (intros _ _ S _;elimT Set.Set_ind S;trivial).
+  mem x xs = mem (f x) (map f xs) by (intros _ _ S _;elimT Set.Set_ind S;smt).
 *)
 
 require List.
+
 
 op remove(x:'a, l:'a List.list) = List.filter (lambda y, x <> y) l.
 
 lemma rem : forall (x:'a) l, List.mem x (remove x l) = false by [].
 
-lemma rem_cons : forall (x:'a) l, !List.mem x l => remove x (List.(::) x l) = l by admit.
+lemma rem_cons : forall (x:'a) l, !List.mem x l => remove x (List.(::) x l) = l.
+intros x l.
+delta remove.
+simplify.
+rewrite (List.filter_cons<:'a> (lambda (y : 'a), !(x = y)) x l).
+simplify.
+elimT List.list_ind l.
+smt.
+simplify.
+intros y xs hrec h.
+rewrite (List.filter_cons<:'a> (lambda (y : 'a), !(x = y)) y xs).
+simplify.
+rewrite (_ : ((!(x = y)) = true));first smt.
+simplify.
+rewrite (hrec _);first smt.
+split.
+save.
+
 
 op enum(s:'a set) : 'a List.list = fold_right List.(::) (List.__nil) s.
 
 pred eq (x y:'a List.list) = forall a, List.mem a x = List.mem a y.
 
-lemma mem_fold_rm : forall x (s:'a set), !(List.mem x (enum (rm x s))).
-intros x s.
-delta enum.
-simplify.
-elimT Induction.induction s.
-trivial.
-simplify.
-intros y S h.
-case (x = y).
-trivial.
-rewrite <- (List.mem_cons<:'a> x (fold_right List.(::) List.__nil (rm x (add y S)))).
-rewrite (fold_rm<:'a List.list, 'a> List.(::) List.__nil (rm x S)).
-
-trivial.
-lemma enum_rm : forall (s:'a set), let x = pick s in eq (enum (rm x s)) (remove x (enum s)).
-intros s.
-delta eq.
-simplify.
-intros a.
-delta enum.
-simplify.
-rewrite (fold_rm<:'a List.list, 'a> List.(::) List.__nil s).
-rewrite (rem_cons<:'a> (pick s) (fold_right List.(::) List.__nil (rm (pick s) s)) _).
-
-admit.
-split.
-save.
-
-
-(*
-lemma fold_set_list : forall (f:'a -> 'b -> 'b) (e:'b) (s:'a set),
-  fold_right f e s = List.fold_right f e (set_to_list s).
-intros f e s.
-elimT Induction.induction_det s;first trivial.
-delta set_to_list.
-simplify.
-intros S h.
-rewrite (fold_rm<:'a List.list,'a> List.(::) List.__nil S).
-rewrite (fold_rm<:'b,'a> f e S).
-rewrite h.
-rewrite (List.fold_right_cons<:'b, 'a> e f (pick S) (fold_right List.(::) List.__nil (rm (pick S) S))).
-split.
-save.
-*)
-
-op sum(f:'a -> real, s:'a set) : real =
-  List.fold_right (lambda (x:'a, sum:real), sum + f x) (0%r) (enum s).
-
-lemma sum_nil:
-  forall (f:'a -> real), sum f Set.empty = 0%r by [].
-
-lemma sum_rm :
-  forall (f:'a -> real) (s:'a set) (x:'a),
-  mem x s =>
-  sum f s = (f x) + (sum f (rm x s)).
-intros f s x h.
-delta sum.
-simplify.
-  apply (Induction.induction
-(lambda S, S <> empty => S <= s => (
-fold_right (lambda (x0 : 'a) (sum : real), sum + f x0) 0%r S =
-f x +
-fold_right (lambda (x0 : 'a) (sum : real), sum + f x0) 0%r (rm x S)
-)) _ _ s _);first trivial.
-simplify.
-intros y S h1 h2 h3 h4.
-trivial.
-
-cut lem : (S <> empty =>
-fold_right (lambda (x0 : 'a) (sum : real), sum + f x0) 0%r S =
-f x +
-fold_right (lambda (x0 : 'a) (sum : real), sum + f x0) 0%r (rm x S)).
-
-elimT Induction.induction S.
-trivial.
-intros x0 S0 hh hhh hhhh.
-trivial.
-
-
-(*
-lemma sum_add :
-  forall (f:'a -> real) (s:'a set) (x:'a),
-  (!mem x s) =>
-  sum f (add x s) = (f x) + (sum f s) by [].
-*)
-
-lemma sum_in :
-  forall (f:'a -> real) (s:'a set),
-  sum f s = sum (lambda x, if mem x s then f x else 0%r) s.
-proof.
-  delta sum.
+lemma mem_enum : forall x (s:'a set), mem x s = List.mem x (enum s).
+  intros x s.
+  elimT Induction.induction_det s.
+  smt.
+  delta enum.
   simplify.
-  intros f s.
-  apply (Induction.induction_det
-(lambda S, S <= s => (
-fold_right (lambda (x : 'a) (sum : real), sum + f x) 0%r S =
-fold_right
-  (lambda (x : 'a) (sum : real), sum + if mem x s then f x else 0%r) 0%r
-  S)
-) _ _ s);first trivial.
-simplify.
-intros S h hh.
-rewrite (fold_rm<:real,'a> (lambda (x : 'a) (sum : real), sum + f x) 0%r S).
-rewrite (fold_rm<:real,'a> (lambda (x : 'a) (sum : real), sum + if mem x s then f x else 0%r) 0%r S).
-simplify.
-rewrite (h _);first trivial.
-cut lem : (mem (pick S) s = true);first trivial.
-rewrite lem.
-simplify.
-split.
+  intros S h.
+  rewrite (fold_rm<:'a List.list, 'a> List.(::) List.__nil S).
+  smt.
 save.
 
-lemma sum_add2 :
-  forall (f:'a -> real) (g:'a -> real) (s:'a set),
-  (sum f s) + (sum g s) = sum (lambda x, f x + g x) s.
-proof.
-intros f g s.
-delta sum.
-elimT Induction.induction_det s;first trivial.
-simplify.
-intros S h.
-rewrite (fold_rm<:real,'a> (lambda (x0 : 'a) (sum : real), sum + f x0) 0%r S).
-rewrite (fold_rm<:real,'a> (lambda (x0 : 'a) (sum : real), sum + g x0) 0%r S).
-rewrite (fold_rm<:real,'a> (lambda (x0 : 'a) (sum : real), sum + (f x0 + g x0)) 0%r S).
-simplify.
-rewrite <- h.
-generalize (fold_right (lambda (x0 : 'a) (sum : real), sum + f x0) 0%r (rm (pick S) S)).
-generalize (fold_right (lambda (x0 : 'a) (sum : real), sum + g x0) 0%r (rm (pick S) S)).
-intros a b.
-trivial.
-save.
+lemma mem_fold_rm : forall x (s:'a set), !(List.mem x (enum (rm x s))) by [].
 
-(*
-lemma map_rm : forall (f:'a->'b) S x, mem x S => (forall y, f y = f x => y = x) => map f (rm x S) = rm (f x) (map f S).
-intros f s x h hh.
-  apply (Induction.induction_det
-(lambda S, S <= s => (
-map f (rm x S) = rm (f x) (map f S)
-)) _ _ s);first trivial.
-simplify.
-intros S hyp hyp2.
-case (x = pick S);first trivial.
-intros neq.
-trivial.
-trivial.
+lemma enum : forall (s t:'a set), s == t <=> eq (enum s) (enum t) by [].
 
-elimT Induction.induction_det S.
-trivial.
-simplify.
-intros S0 hyp.
-
-delta map.
-simplify.
-*)
-
-lemma sum_chind :
-  forall (f:'a -> real) (g:'a -> 'a) (gg:'a -> 'a) (s:'a set),
-    (forall x, g (gg x) = x /\ gg (g x) = x) => (*TROP FORT ?*)
-  (sum f s) = sum (lambda x, f (gg x)) (map g s).
-proof.
+lemma enum_rm : forall (s:'a set) x, eq (enum (rm x s)) (remove x (enum s)).
 admit.
-(*
-intros f g gg s bij.
-delta sum.
-simplify.
-rewrite (fold_set_list<:real, 'a> (lambda (x : 'a) (sum : real), sum + f x) 0%r s).
-rewrite (fold_set_list<:real, 'a> (lambda (x : 'a) (sum : real), sum + f (gg x)) 0%r (map g s)).
-rewrite <- (map_set_list<:'a, 'a> g s).
-elimT List.list_ind (set_to_list s);first trivial.
-simplify.
-intros x xs h.
-rewrite (List.map_cons<:'a, 'a> g x xs).
-rewrite (List.fold_right_cons<:real, 'a> 0%r (lambda (x0 : 'a) (sum : real), sum + f x0) x xs).
-rewrite (List.fold_right_cons<:real, 'a> 0%r (lambda (x0 : 'a) (sum : real), sum + f (gg x0)) (g x) (List.map g xs)).
-simplify.
-rewrite h.
-rewrite (_ : f (gg (g x)) = f x);first trivial.
-split.
-*)
+save.
+
+lemma rem_cons2 : forall (x:'a) l, List.mem x l => eq (List.(::) x (remove x l)) l.
+delta eq.
+smt.
+save.
+
+lemma exist : forall (l:'a List.list), exists (s:'a set), enum s = l.
+admit.
 save.
