proof/garble/clonesMean.ec
@@ -1,0 +1,197 @@
+require import Set.
+require import Int.
+require import Bool.
+require import Distr.
+require import Real.
+
+require import MySum.
+require import MyInt.
+
+require import CloneDkc.
+require import Garble.
+require import Mean.
+require import AdvGarbleAda.
+
+clone Mean as MeanBool with
+  type base = bool,
+  op d = Dbool.dbool,
+  op support = Set.add false (Set.add true Set.empty).
+
+clone Mean as MeanInt with
+  type base = int,
+  op d = Dinter.dinter 0 (borne-1),
+  op support = integers 0 borne.
+
+module DkcWorkAdv(Adv:AdvAda_t) = {
+  module Game = DKC.GameAda(DKC.Dkc, Adv)
+  module ADV = Adv(DKC.Dkc)
+  fun work() : bool = {
+    var r : bool;
+    ADV.preInit();
+    r = Game.work();
+    return r;
+  }
+}.
+
+module DkcWork(Adv:DKC.AdvAda_t) : MeanBool.Worker = {
+  module Game = DKC.GameAda(DKC.Dkc, Adv)
+  module ADV = Adv(DKC.Dkc)
+  fun work(x:bool) : bool = {
+    var r : bool;
+    DKC.Dkc.b = x;
+    ADV.preInit();
+    r = Game.work();
+    return r;
+  }
+}.
+
+lemma DkcExp : forall (M<:DKC.Exp),
+  equiv[M.work~M.work:(glob M){1}=(glob M){2}==>res{1}=res{2}].
+proof.
+intros _;fun true;progress assumption.
+save.
+
+
+lemma DkcWork :
+  forall b,
+  forall &m,
+    forall (Adv<:DKC.AdvAda_t {DKC.Dkc, DKC.Game}),
+      DKC.Dkc.b{m} = b =>
+  Pr[DkcWorkAdv(Adv).work()@ &m:res] = 
+    Pr[DkcWork(Adv).work(b)@ &m:res].
+proof.
+  intros b &m Adv h.
+  cut eq : equiv[DkcWorkAdv(Adv).work ~ DkcWork(Adv).work
+: DKC.Dkc.b{1} = x{2} /\ (glob Adv){1} = (glob Adv){2} /\ (glob DKC.GameAda(DKC.Dkc,Adv)){1} = (glob DKC.GameAda(DKC.Dkc,Adv)){2}
+      ==>res{1}=res{2}].
+  fun.
+  call ((glob DKC.GameAda(DKC.Dkc,Adv)){1} = (glob DKC.GameAda(DKC.Dkc,Adv)){2}) (res{1}=res{2}).
+  apply (DkcExp (<:DKC.GameAda(DKC.Dkc,Adv))).
+  call ((glob Adv){1} = (glob Adv){2}) (res{1}=res{2}/\(glob Adv){1} = (glob Adv){2}).
+  fun true;progress assumption.
+  wp.
+  skip;progress.
+  equiv_deno eq;progress assumption.
+save.
+
+lemma DkcEsp :
+  forall &m,
+    forall (Adv<:DKC.AdvAda_t {DKC.Dkc, DKC.Game}),
+      Pr[DKC.GameAda(DKC.Dkc, Adv).main()@ &m:res] = 
+        (Pr[DkcWork(Adv).work(true)@ &m:res] +
+           Pr[DkcWork(Adv).work(false)@ &m:res]) / 2%r.
+proof.
+  intros &m Adv.
+  cut pr : (Pr[DKC.GameAda(DKC.Dkc, Adv).main()@ &m:res] = Pr[MeanBool.Rand(DkcWork(Adv)).randAndWork()@ &m:res]).
+    cut eq : equiv[
+      DKC.GameAda(DKC.Dkc, Adv).main ~
+      MeanBool.Rand(DkcWork(Adv)).randAndWork: (glob Adv){1} = (glob Adv){2}/\ (glob DKC.GameAda(DKC.Dkc, Adv)){1}=(glob DKC.GameAda(DKC.Dkc, Adv)){2}
+      ==>res{1}=res{2}].
+      fun.
+      inline DKC.GameAda(DKC.Dkc, Adv).preInit.
+      inline DKC.Dkc.preInit.
+      inline DkcWork(Adv).work.
+      wp.
+      cut prelem : (forall (M<:DKC.Exp), equiv[M.work~M.work:(glob M){1}=(glob M){2}==>res{1}=res{2}]);
+        first (intros M;fun true;by progress).
+      call ((glob DKC.GameAda(DKC.Dkc, Adv)){1}=(glob DKC.GameAda(DKC.Dkc, Adv)){2}) (res{1}=res{2});
+        first apply (prelem (<:DKC.GameAda(DKC.Dkc, Adv))).
+      wp.
+      call ((glob Adv){1} = (glob Adv){2}) ((glob Adv){1} = (glob Adv){2});first (fun true;by progress).
+      wp;rnd;skip;by (progress assumption).
+    equiv_deno eq;progress assumption;smt.
+  rewrite pr.
+  rewrite (MeanBool.Mean &m (<:DkcWork(Adv))).
+  delta MeanBool.support.
+  rewrite (sum_add<:bool> (lambda (x : MeanBool.base),
+     mu_x MeanBool.d x * Pr[DkcWork(Adv).work(x) @ &m : res{hr}]) (add true Set.empty) false _);first smt.
+  rewrite (sum_add<:bool> (lambda (x : MeanBool.base),
+     mu_x MeanBool.d x * Pr[DkcWork(Adv).work(x) @ &m : res{hr}]) Set.empty true _);first smt.
+  rewrite (sum_nil<:bool> (lambda (x : MeanBool.base),
+     mu_x MeanBool.d x * Pr[DkcWork(Adv).work(x) @ &m : res{hr}])).
+  simplify.
+  delta MeanBool.d.
+  rewrite (Dbool.mu_x_def false).
+  rewrite (Dbool.mu_x_def true).
+  smt.
+save.
+
+theory AdvEsp.
+
+  op b : bool.
+
+  module AdvWork(Adv:Garble.Adv) : MeanInt.Worker = {
+    (*TODO*)
+    module Game = GameAda(DKC.Dkc, Adv)
+
+    fun work(x:int) : bool = {
+      var r : bool;
+      AdvAda.l = x;
+      DKC.Dkc.b = b;
+      r = Game.work();
+      return r;
+    }
+}.
+
+lemma RemAdvEsp : forall (ADV <: Garble.Adv{AdvAda}),
+  forall &1 &2 x, DKC.Dkc.b{1} = b => AdvAda.l{2} = x =>
+    Pr[AdvWork(ADV).work(x) @ &1 : res] =
+      Pr[GameAda(DKC.Dkc, ADV).work() @ &2 : res].
+  admit.
+save.
+
+lemma AdvEsp :
+  forall &m,
+    forall (Adv<:Garble.Adv{DKC.Dkc,AdvAda,DKC.Game}),
+      forall c, c = b =>
+      Pr[DkcWork(AdvAda(Adv,DKC.Dkc)).work(c)@ &m:res] =
+        (sum (lambda l, (1%r / borne%r) * Pr[AdvWork(Adv).work(l)@ &m:res]) MeanInt.support).
+proof.
+  intros &m Adv c h.
+  cut pr : (Pr[MeanInt.Rand(AdvWork(Adv)).randAndWork()@ &m:res] = Pr[DkcWork(AdvGarble.Adv(Adv)).work(c)@ &m:res]).
+    cut eq : equiv[
+      MeanInt.Rand(AdvWork(Adv)).randAndWork ~
+      DkcWork(AdvGarble.Adv(Adv)).work: x{2} = c /\ (glob DKC.Game(DKC.Dkc, AdvGarble.Adv(Adv))){1}=(glob DKC.Game(DKC.Dkc, AdvGarble.Adv(Adv))){2}
+      ==>res{1}=res{2}].
+      fun.
+      inline AdvGarble.Adv(Adv).preInit.
+      inline AdvWork(Adv).work.
+      wp.
+      call ((glob DKC.Game(DKC.Dkc, AdvGarble.Adv(Adv))){1}=(glob DKC.Game(DKC.Dkc, AdvGarble.Adv(Adv))){2}) (res{1}=res{2}).
+      apply (DkcExp (<:DKC.Game(DKC.Dkc, AdvGarble.Adv(Adv)))).
+      wp.
+      rnd.
+      wp.
+      skip;progress assumption.
+    equiv_deno eq;progress assumption;smt.
+  rewrite <- pr.
+
+rewrite (sum_in<:int> (lambda (l : int), (1%r / borne%r) * Pr[AdvWork(Adv).work(l) @ &m : res{hr}]) MeanInt.support).
+simplify.
+cut lem : ((lambda (x:int),
+(if mem x MeanInt.support then
+  1%r / borne%r * Pr[AdvWork(Adv).work(x) @ &m : res{hr}]
+else
+  0%r)) = lambda (x:int), (mu_x MeanInt.d x * Pr[AdvWork(Adv).work(x) @ &m :res{hr}])).
+delta MeanInt.d.
+apply (Fun.extensionality<:real, int> (lambda (x:int),
+(if mem x MeanInt.support then
+  1%r / borne%r * Pr[AdvWork(Adv).work(x) @ &m : res{hr}]
+else
+  0%r)) (lambda (x:int), (mu_x MeanInt.d x * Pr[AdvWork(Adv).work(x) @ &m :res{hr}])) _).
+intros x.
+case (mem x MeanInt.support = true);last smt.
+intros hh.
+delta MeanInt.d.
+rewrite (Dinter.mu_x_def_in 0 (borne-1) x _);first smt.
+rewrite (_:((borne - 1) - 0) + 1 = borne);first smt.
+rewrite hh.
+progress.
+rewrite lem.
+apply (MeanInt.Mean &m (<:AdvWork(Adv))).
+save.
+
+end AdvEsp.
+
+clone AdvEsp as AdvEspTrue with op b = true.
+clone AdvEsp as AdvEspFalse with op b = false.
