proof/garble/endProof.ec
@@ -1,0 +1,217 @@
+require import Real.
+
+lemma math :
+forall (x:real) (b:int),
+x =
+2%r * b%r *
+((1%r / b%r * x + 1%r / b%r * (1%r / 2%r) + (b%r - 1%r) * (1%r / b%r)) / 2%r) +
+1%r / 2%r - b%r.
+smt "Mathematica".
+save.
+
+require import Int.
+
+lemma simpl : (forall (x y z:real), y>0%r=> x < z  => x * y < y * z) by [].
+
+require import Fun.
+require import Set.
+
+require import MySum.
+require import MyInt.
+
+require AdvGarble.
+require import Garble.
+require import ClonesMean.
+require import CloneDkc.
+
+(*
+require import Bitstring.
+require import List.
+require import Map.
+require import Set.
+require import Pair.
+require import Bool.
+require import Distr.
+require import Fun.
+require import Logic.
+
+require import MyTools.
+require import Garble.
+require import GarbleTools.
+require import Myset.
+require import MyMean.
+*)
+
+lemma prReal :
+  forall (ADV <: Garble.Adv{AdvGarble.Adv}),
+    forall &m,
+    Pr[AdvEspTrue.AdvWork(ADV).work(0) @ &m : res] =
+      Pr[Garble.Game(Garble.PrvInd(RandGarble), ADV).main() @ &m : res].
+proof.
+  rewrite (AdvEspTrue.RemAdvEsp
+
+save.
+
+lemma prHybrid :
+  forall (ADV <: Garble.Adv{AdvGarble.Adv}),
+    forall &m x,
+      x >= 0 /\ x < borne =>
+    let y = x + 1 in
+    Pr[AdvEspFalse.AdvWork(ADV).work(x) @ &m : res] =
+      Pr[AdvEspTrue.AdvWork(ADV).work(y) @ &m : !res].
+proof.
+  admit.
+save.
+
+lemma prFake :
+  forall (ADV <: Garble.Adv{AdvGarble.Adv}),
+    forall &1,
+        let x = borne - 1 in
+        Pr[AdvEspFalse.AdvWork(ADV).work(x)@ &1 : res] = 1%r / 2%r.
+proof.
+  admit.
+save.
+
+lemma RelDkcGarble :
+  forall &m,
+    forall (Adv<:Garble.Adv{DKC.Dkc,DKC.Game,AdvGarble.Adv}),
+      Pr[Garble.Game(Garble.PrvInd(RandGarble), Adv).main()@ &m:res] =
+        2%r * borne%r * Pr[GameAda(DKC.Dkc, ADV).work()@ &m:res]
+          + 1%r / 2%r - borne%r.
+proof.
+  intros &m Adv.
+  rewrite (DkcEsp &m (<:AdvGarble.Adv(Adv))).
+  rewrite (AdvEspTrue.AdvEsp &m (<:Adv) true).
+  rewrite (AdvEspFalse.AdvEsp &m (<:Adv) false).
+
+(**Remove Pr*)
+  cut introF : (exists (f:int->real), (forall (l:int), (f l) =
+    Pr[AdvEspTrue.AdvWork(Adv).work(l) @ &m : res{hr}]));first
+    (exists (lambda (l:int), Pr[AdvEspTrue.AdvWork(Adv).work(l) @ &m : res{hr}]);
+     simplify;split).
+  elim introF.
+  intros f fv.
+  rewrite (_:(lambda (l : int),
+       1%r / borne%r *
+       Pr[AdvEspTrue.AdvWork(Adv).work(l) @ &m : res{hr}]) = lambda (l : int),
+       1%r / borne%r * (f l));
+    first (apply Fun.extensionality;delta Fun.(==);simplify;intros l;rewrite (fv l);split).
+(**End Remove Pr*)
+
+(**Remove Pr*)
+  cut introG : (exists (g:int->real), (forall (l:int), (g l) =
+    Pr[AdvEspFalse.AdvWork(Adv).work(l) @ &m : res{hr}]));first
+    (exists (lambda (l:int), Pr[AdvEspFalse.AdvWork(Adv).work(l) @ &m : res{hr}]);
+     simplify;split).
+  elim introG.
+  intros g gv.
+  rewrite (_:(lambda (l : int),
+       1%r / borne%r *
+       Pr[AdvEspFalse.AdvWork(Adv).work(l) @ &m : res{hr}]) = lambda (l : int),
+       1%r / borne%r * (g l));
+    first (apply Fun.extensionality;delta Fun.(==);simplify;intros l;rewrite (gv l);split).
+(**End Remove Pr*)
+
+(**Remove Pr*)
+cut valf0 : (f 0 = Pr[Game(PrvInd(RandGarble), Adv).main() @ &m : res{hr}]).
+  rewrite (fv 0).
+  apply (prReal (<:Adv) &m).
+rewrite <- valf0.
+(**End Remove Pr*)
+
+  rewrite (sum_rm<:int>
+   (lambda (l : int), 1%r / borne%r * (f l))
+   MeanInt.support
+   0 _);first smt.
+  rewrite (sum_rm<:int>
+   (lambda (l : int), 1%r / borne%r * (g l))
+   MeanInt.support
+   (borne-1) _);first smt.
+simplify.
+rewrite ( _ :
+1%r / borne%r * f 0 +
+  sum (lambda (l : int), 1%r / borne%r * f l)
+    (rm 0 MeanInt.support) +
+  (1%r / borne%r * g (borne-1) +
+   sum (lambda (l : int), 1%r / borne%r * g l)
+     (rm (borne-1) MeanInt.support))
+=
+1%r / borne%r * (f 0) +
+1%r / borne%r * (g (borne-1)) +
+(
+sum (lambda (l : int), 1%r / borne%r * (f l)) (rm 0 MeanInt.support) +
+sum (lambda (l : int), 1%r / borne%r * (g l)) (rm (borne-1) MeanInt.support)
+)
+);first smt.
+
+  rewrite (sum_chind<:int>
+    (lambda (l : int),
+       1%r / borne%r * (f l))
+    (lambda (x:int), x - 1)
+    (lambda (x:int), x + 1)
+    (rm 0 MeanInt.support) _);first smt.
+  simplify.
+  delta MeanInt.support.
+  rewrite (dec_integers 0 borne _);first smt.
+  rewrite (sum_add2<:int>
+    (lambda (l : int), 1%r / borne%r * f (l+1))
+    (lambda (l : int), 1%r / borne%r * g l)
+    (rm (borne-1) (integers 0 borne))).
+  simplify.
+  cut lem : (forall x, mem x (rm (borne-1) (integers 0 borne)) =>
+    f (Int.(+) x 1) = 1%r - g x).
+      intros x h.
+      rewrite (fv (x+1)).
+      rewrite (gv x).
+      rewrite (prHybrid (<:Adv) &m x _);first smt.
+      apply (MeanInt.Not &m (<:AdvEspTrue.AdvWork(Adv)) (x + 1)).
+    
+  rewrite (sum_in<:int> (lambda (x : int),
+       1%r / borne%r * f (Int.(+) x 1) +
+       1%r / borne%r * g x) (rm (borne-1) (integers 0 borne))).
+  simplify.
+  rewrite (_ : (lambda (x:int),
+(if mem x (rm (borne-1) (integers 0 borne)) then
+         1%r / borne%r * f (Int.(+) x 1) +
+         1%r / borne%r * g x
+       else 0%r))
+= (lambda (x:int), if mem x (rm (borne-1) (integers 0 borne)) then 1%r / borne%r else 0%r)
+);first (apply Fun.extensionality;smt).
+  rewrite (sum_const<:int> (1%r/borne%r)
+(lambda (x : int),
+       if mem x (rm (Int.(-) borne 1) (integers 0 borne)) then 1%r / borne%r
+       else 0%r)
+(rm (Int.(-) borne 1) (integers 0 borne))
+_
+);first smt.
+cut valgborne : (g (borne-1) = 1%r / 2%r).
+  rewrite (gv (borne-1)).
+  apply (prFake (<:Adv) &m).
+rewrite valgborne.
+rewrite (_:(card (rm (Int.(-) borne 1) (integers 0 borne)))%r = borne%r - 1%r).
+smt.
+apply math.
+save.
+
+lemma PrvIndGarble :
+  exists (epsilon:real), epsilon > 0%r /\
+    forall (Adv<:Garble.Adv{DKC.Dkc,DKC.Game,AdvGarble.Adv}), forall &m,
+        `|Pr[Garble.Game(Garble.PrvInd(RandGarble), Adv).main()@ &m:res] - 1%r / 2%r| < epsilon.
+proof.
+  elim DKC.Security.
+  intros epDkc hDkc.
+  elim hDkc. clear hDkc.
+  intros hPos hDkc.
+  exists (borne%r*epDkc).
+  cut bPos : (borne%r > 0%r);first smt.
+  progress;first smt.
+  rewrite (RelDkcGarble &m (<:Adv)).
+  cut remPr : (forall (x:real), `|2%r * x - 1%r| < epDkc => `|2%r * borne%r * x +
+  1%r / 2%r - borne%r - 1%r / 2%r| < borne%r * epDkc).
+    intros x h.
+    rewrite (_:`|2%r * borne%r * x + 1%r / 2%r - borne%r - 1%r / 2%r| = `|2%r * x - 1%r| * `| borne%r|);first smt.
+  rewrite (_:(`|borne%r| = borne%r));first smt.
+  apply (simpl (`|2%r * x - 1%r|) (borne%r) epDkc);assumption.
+  apply (remPr Pr[DKC.Game(DKC.Dkc, AdvGarble.Adv(Adv)).main() @ &m :res{hr}] _).
+  apply (hDkc (<:AdvGarble.Adv(Adv)) &m).
+save.
