proof/garble/equivFake.ec
@@ -1,0 +1,322 @@
+require import Bitstring.
+require import List.
+require import Map.
+require import Set.
+require import Pair.
+require import Real.
+require import Int.
+require import Bool.
+require import Array.
+require import Distr.
+
+require import CloneDkc.
+require import GarbleTools.
+require import Garble.
+require import AdvGarbleAda.
+
+module Fake(A:Garble.Adv) = {
+
+  var f1 : Garble.funct
+  var x1 : Garble.input
+  var good : bool
+  var tau : bool
+  var queries : DKC.query array
+  var ans : DKC.answer array
+  var answer : Garble.functG*Garble.inputG*Garble.keyOutput
+  var query : Garble.query
+
+  var n : int
+  var m : int
+  var q : int
+  var aa : w2g
+  var bb : w2g
+  var pp : token g2v
+  var t : bool array
+  var v : bool array
+  var xx : tokens
+  var a : int
+  var b : int
+  var i : int
+  var g : int
+
+(*DKC var*)
+  var ksec : token
+  var r : (int*bool, token) map
+  var kpub : (int*bool, token) map
+(*End DKC Var*)
+
+  fun query(rand:bool, alpha:bool, bet:bool) : token = {
+    var ttt : token;
+    var pos : bool;
+    var input : int*bool;
+    var output : int*bool;
+    var ra : bool;
+    var ki : token;
+    var ko : token;
+    var zz : token;
+
+    ttt = tweak g (t.[a]^^alpha) (t.[b]^^bet);
+    input = (a, (t.[a]^^alpha));
+    if (rand) {
+      ra = $Dbool.dbool;
+      output = (g + n + q, ra);
+    } else
+      output = (g, true (*TODO (evalGate gg.[g] ((v.[a]^^alpha),(v.[b]^^bet)))*));
+
+
+
+    (*DKC encrypt*)
+        if (! (in_dom input kpub)) kpub.[input] = $DKC.genRandKeyLast (snd input);
+        if (! (in_dom output kpub)) kpub.[output] = $DKC.genRandKeyLast (snd output);
+        if (! (in_dom output r)) r.[output] = $DKC.genRandKey;
+        ki = proj kpub.[input];
+        ko = proj kpub.[output];
+        zz = DKC.encode ttt (proj kpub.[input]) ksec (proj r.[output]);
+    (*End DKC encrypt*)
+     
+
+
+
+
+
+
+    ans = sub ans 0 ((length ans) - 1);
+    pp.[g] = setGateVal pp.[g] ((t.[a]^^alpha), (t.[b]^^bet)) zz;
+    xx = setTok xx g (v.[a]^^alpha) ki;
+    return ko;
+  }
+
+  fun garb(yy:token, alpha:bool, bet:bool) : unit = {
+    pp.[g] = setGateVal pp.[g] ((t.[a]^^alpha), (t.[b]^^bet)) (DKC.encode
+      (tweak g (t.[a]^^alpha) (t.[b]^^bet))
+      (getTok xx a (v.[a]^^alpha))
+      (getTok xx b (v.[b]^^alpha))
+      yy);
+  }
+
+  fun garbD(alpha:bool, bet:bool) : token = {
+    var yy : token;
+    yy = $DKC.genRandKey;
+    garb(yy, alpha, bet);
+    return yy;
+  }
+
+  fun garble() : unit = {
+    var tok : token;
+    var yyt : token;
+
+    i = 0;
+    while (i < n+q-m) {
+      v.[i] = eval f1 x1 i;
+      t.[i] = $Dbool.dbool;
+      i = i + 1;
+    }
+    while (i < n+q) {
+      v.[i] = eval f1 x1 i;
+      t.[i] = false;
+      i = i + 1;
+    }
+
+
+    t.[borne-1] = !tau;
+
+    g = n;
+    while (g < n+q) {
+      a = aa.[g];
+      b = bb.[g];
+      if (b = borne - 1) {
+        tok = query(false, false, true);
+        tok = query(true, true, true);
+      }
+      g = g + 1;
+    }
+
+    i = 0;
+    while (i < n+q) {
+      if (getTok xx i true = void /\ i <> 0) {
+        tok = $DKC.genRandKeyLast (! t.[i]);
+        xx = setTok xx i true tok;
+      }
+      if (getTok xx i false = void) {
+        tok = $DKC.genRandKeyLast (t.[i]);
+        xx = setTok xx i false tok;
+      }
+      i = i + 1;
+    }
+
+    g = n;
+    while (g < n+q) {
+      a = aa.[g];
+      b = bb.[g];
+      garb(getTok xx g v.[g], false, false);
+      if (b <> borne - 1) {
+        tok = garbD(true, false);
+        tok = garbD(false, true);
+        tok = garbD(true, true);
+      } else {
+        tok = garbD(true, false);
+      }
+      g = g + 1;
+    }
+    answer = ((getN f1, getM f1, getQ f1, getA f1, getB f1, pp), encrypt (Array.sub xx 0 (getN f1)) x1,tt);
+  }
+
+  fun work() : bool = {
+    var challenge : bool;
+    var c : bool;
+    var ret : bool;
+    var gg : bool g2v;
+
+    query = A.gen_query();
+  
+    if (Garble.queryValid query)
+    {
+      tau = $Dbool.dbool;
+      ksec = $DKC.genRandKeyLast tau;
+      kpub = Map.empty;
+      r = Map.empty;
+
+      (f1, x1) = fst query;
+      (n, m, q, aa, bb, gg) = f1;
+      queries = Array.empty;
+      t = Array.init (n+q) false;
+      v = Array.init (n+q) false;
+      xx = Array.init (n+q) (void, void);
+      pp = Array.init (n+q) (void, void, void, void);
+      garble();
+      challenge = A.get_challenge(answer);
+      c = $Dbool.dbool;
+      ret = (c = challenge);
+    }
+    else
+      ret = $Dbool.dbool;
+    return ret = false;
+  }
+
+}.
+
+
+lemma fakeEq :
+  forall (ADV <: Garble.Adv{AdvAda, DKC.Dkc, Fake}),
+    equiv [
+      GameAda(DKC.Dkc, ADV).work ~
+      Fake(ADV).work
+      : (glob ADV){1} = (glob ADV){2} /\
+      (!DKC.Dkc.b{1}) /\ (AdvAda.l{1}=borne-1) ==> res{1} = res{2}
+    ].
+proof.
+  intros ADV.
+  fun.
+  inline {1} GameAda(DKC.Dkc, ADV).A.work.
+  inline {1} AdvAda(ADV, DKC.Dkc).work.
+  inline {1} AdvAda(ADV, DKC.Dkc).garble.
+  inline {1} AdvAda(ADV, DKC.Dkc).query.
+  inline {1} AdvAda(ADV, DKC.Dkc).garbD.
+  inline {1} AdvAda(ADV, DKC.Dkc).garb.
+  inline {1} DKC.Dkc.preInit.
+  inline {1} DKC.Dkc.get_challenge.
+  inline {1} DKC.Dkc.initialize.
+  inline {1} DKC.Dkc.encrypt.
+  inline {2} Fake(ADV).work.
+  inline {2} Fake(ADV).garble.
+  inline {2} Fake(ADV).query.
+  inline {2} Fake(ADV).garbD.
+  inline {2} Fake(ADV).garb.
+
+  swap{1} 8 -7.
+
+  seq 1 1 : ((glob ADV){1} = (glob ADV){2}/\AdvAda.query{1} = Fake.query{2} /\ (!DKC.Dkc.b{1}) /\ (AdvAda.l{1}=borne-1)).
+    call ((glob ADV){1} = (glob ADV){2}) (res{1}=res{2} /\ (glob ADV){1} = (glob ADV){2});first (fun true;by progress).
+  skip;progress;assumption.
+  
+  case (Garble.queryValid Fake.query{2}).
+
+  (*VALID*)
+  rcondt {1} 18;first (intros _;wp;rnd;wp;rnd;rnd;skip;progress assumption).
+  rcondt {2} 1;first (intros &m;skip;by progress).
+
+  swap{1} 8 -7.
+  swap{2} 24 -23.
+
+  wp.
+  call ((glob ADV){1} = (glob ADV){2}/\answer{1}=answer{2}) (res{1}=res{2});first (fun true;by progress).
+  wp.
+
+  while (
+    (glob ADV){1} = (glob ADV){2} /\
+    length AdvAda.xx{1} = AdvAda.n{1}+AdvAda.q{1} /\
+    length AdvAda.t{1} = AdvAda.n{1}+AdvAda.q{1} /\
+    AdvAda.xx{1} = Fake.xx{2} /\
+    AdvAda.t{1} = Fake.t{2}/\
+    AdvAda.v{1} = Fake.v{2}/\
+    AdvAda.n{1} = Fake.n{2}/\
+    AdvAda.m{1} = Fake.m{2}/\
+    AdvAda.q{1} = Fake.q{2}/\
+    AdvAda.aa{1} = Fake.aa{2}/\
+    AdvAda.bb{1} = Fake.bb{2}/\
+    AdvAda.fc{1} = Fake.f1{2}/\
+    (AdvAda.c{1} = DKC.Dkc.b{1}) = PrvInd.b{2}/\
+    AdvAda.xc{1} = Fake.x1{2}/\
+    (*Fake.f1{2} = (Fake.n{2}, Fake.m{2}, Fake.q{2}, Fake.aa{2}, Fake.bb{2}, Fake.gg{2}) /\*)
+    borne = Fake.n{2} + Fake.q{2} /\
+    AdvAda.l{1} = borne-1 /\
+    (forall i, i >= Fake.n{2} => i < Fake.n{2}+Fake.q{2} => Fake.aa{2}.[i] >= 0 /\
+           Fake.bb{2}.[i] < borne /\ Fake.bb{2}.[i] < i /\ Fake.aa{2}.[i] < Fake.bb{2}.[i]) /\
+
+    AdvAda.g{1} = Fake.g{2} /\
+      Fake.g{2} > Fake.n{2} /\
+    AdvAda.pp{1} = Fake.pp{2} /\
+    true
+  ).
+    wp.
+    
+    seq 6 6 : (
+      (glob ADV){1} = (glob ADV){2} /\
+      length AdvAda.xx{1} = AdvAda.n{1}+AdvAda.q{1} /\
+      length AdvAda.t{1} = AdvAda.n{1}+AdvAda.q{1} /\
+      AdvAda.xx{1} = Fake.xx{2} /\
+      AdvAda.t{1} = Fake.t{2}/\
+      AdvAda.v{1} = Fake.v{2}/\
+      AdvAda.n{1} = Fake.n{2}/\
+      AdvAda.m{1} = Fake.m{2}/\
+      AdvAda.q{1} = Fake.q{2}/\
+      AdvAda.aa{1} = Fake.aa{2}/\
+      AdvAda.bb{1} = Fake.bb{2}/\
+      AdvAda.fc{1} = Fake.f1{2}/\
+      (AdvAda.c{1} = DKC.Dkc.b{1}) = PrvInd.b{2}/\
+      AdvAda.xc{1} = Fake.x1{2}/\
+      (*Fake.f1{2} = (Fake.n{2}, Fake.m{2}, Fake.q{2}, Fake.aa{2}, Fake.bb{2}, Fake.gg{2}) /\*)
+      borne = Fake.n{2} + Fake.q{2} /\
+      AdvAda.l{1} = borne-1 /\
+    (forall i, i >= Fake.n{2} => i < Fake.n{2}+Fake.q{2} => Fake.aa{2}.[i] >= 0 /\
+           Fake.bb{2}.[i] < borne /\ Fake.bb{2}.[i] < i /\ Fake.aa{2}.[i] < Fake.bb{2}.[i]) /\
+
+
+      AdvAda.g{1} = Fake.g{2} /\
+      Fake.g{2} > Fake.n{2} /\
+      AdvAda.a{1} = Fake.a{2} /\
+      AdvAda.b{1} = Fake.b{2} /\
+      AdvAda.a{1} < borne-1 /\
+      AdvAda.b{1} <= borne-1 /\
+      true
+    );first (wp;skip;progress assumption;smt).
+    if;first smt.
+      (*IF TRUE*)
+      rcondt{1} 4;first (intros _;wp;skip;smt).
+      rcondt{1} 13;first (intros _;wp;rnd;wp;skip;smt).
+      rcondt{1} 22;first (intros _;wp;rnd;wp;rnd;wp;skip;smt).
+      wp;rnd;wp;rnd;wp;rnd;wp;skip;progress assumption;[smt| |smt| ].
+      congr. (*BUG*)
+      (*IF FALSE*)
+      rcondf{1} 1;first (intros _;skip;smt).
+      rcondt{1} 4;first (intros _;wp;skip;smt).
+      wp;rnd;wp;skip;progress assumption;smt.
+
+  (*INVALID*)
+  rcondf {1} 18;first (intros _;wp;rnd;wp;rnd;rnd;skip;smt).
+  rcondf {2} 1;[intros &m;skip;smt|].
+  wp.
+  kill{1} 1!17;first (wp;rnd 1%r cPtrue;wp;rnd 1%r cPtrue;rnd 1%r cPtrue;skip;progress;smt).
+  rnd.
+  skip;progress;smt.
+save.
