proof/myInt.ec
@@ -1,0 +1,55 @@
+require import Set.
+require import Int.
+
+op integers : int -> int -> int set.
+axiom integers_neg : forall (x y:int), x >= y => integers x y = Set.empty.
+axiom integers_pos : forall (x y:int), x < y => integers x y = add (y-1) (integers x (y-1)).
+
+lemma integers : forall (x y a:int), (Set.mem a (integers x y)) <=> (x <= a /\ a < y).
+  intros x y a.
+  case (x < y);last smt.
+  rewrite (_ : y = (y-x)+x);first smt.
+  intros pos.
+  apply (Int.Induction.induction
+    (lambda i, mem a (integers x (i+x)) <=> Int.(<=) x a /\ Int.(<) a (i+x))
+    _ _ (y-x) _);[smt| |smt].
+  simplify.
+  intros j h hrec.
+  rewrite (integers_pos x (j+x) _);smt.
+save.
+
+lemma dec_integers : forall (x y:int),
+    x < y =>
+    (map (lambda (x : int), x-1) (rm x (integers x y)) =
+    (rm (y-1) (integers x y))
+    ).
+  intros x y h.
+  apply Set.extensionality.
+  delta Set.(==).
+  simplify.
+  intros a.
+  rewrite (_:rm x (integers x y) = integers (x+1) y);
+    first (apply Set.extensionality;delta Set.(==);smt).
+  rewrite (_:rm (y-1) (integers x y) = integers x (y-1));
+    first (apply Set.extensionality;delta Set.(==);smt).
+  apply iff_intro.
+  intros hh.
+  elim (mem_map_rev<:int,int> (lambda (x0 : int), Int.(-) x0 1) (integers (x+1) y) (a+1) _);
+    first (simplify;rewrite (_:(Int.(-) (Int.(+) a 1) 1) = a));smt.
+  intros hh.
+  rewrite <- (_:(Int.(-) (Int.(+) a 1) 1) = a);first smt.
+  apply (mem_map<:int,int> (lambda (x0 : int), Int.(-) x0 1) (integers (x+1) y) (a+1) _).
+  smt.
+save.
+
+lemma card_integers : forall x y, card (integers x y) = max (y - x) 0.
+  intros x y.
+  case (x < y);last smt.
+  intros h.
+  rewrite (_:integers x y=integers x (x+(y-x)));first smt.
+  rewrite (_:max (y - x) 0 = y-x);first smt.
+  apply (Int.Induction.induction (lambda i, card (integers x (x+i)) = i) _ _ (y-x) _);[smt| |smt].
+  simplify.
+  intros j hh hrec.
+  rewrite (integers_pos x (x+j) _);smt.
+save.
